LeanFM/LLMGenerated/Implementation.lean
@@ -1,0 +1,55 @@
+import LeanFM.LLMGenerated.Requirements
+
+namespace LeanFM.LLMGenerated.Implementation
+
+open LeanFM.LLMGenerated.Requirements
+
+def actorBinding : WorkerActor -> LeanFM.ActorCodegen
+  | .Client => { actor := LeanFM.requirementName WorkerActor.Client
+               , typeName := "ClientActor", sourceFile := "internal/actors/client.go" }
+  | .Gateway => { actor := LeanFM.requirementName WorkerActor.Gateway
+                , typeName := "GatewayActor", sourceFile := "internal/actors/gateway.go" }
+  | .Worker => { actor := LeanFM.requirementName WorkerActor.Worker
+               , typeName := "WorkerActor", sourceFile := "internal/actors/worker.go" }
+
+def messageBinding (message : LeanFM.MessageSchema) : LeanFM.MessageCodegen :=
+  { message := message.name
+  , wireType := "pb." ++ LeanFM.replaceChar '.' '_' message.name
+  , transport :=
+      match message.name with
+      | "Docs.GetRequest" => .httpRequest "GET" "/docs/{path}"
+      | "Docs.FetchCommand" => .httpRequest "POST" "/internal/docs/fetch"
+      | "Docs.FetchResult200" => .httpResponse "Docs.FetchCommand"
+      | "Docs.FetchResult404" => .httpResponse "Docs.FetchCommand"
+      | "Docs.GetResponse" => .httpResponse "Docs.GetRequest"
+      | "Error.Response" => .httpResponse "Docs.GetRequest"
+      | "Reviews.PostRequest" => .httpRequest "POST" "/reviews"
+      | "Reviews.ModerateCommand" => .httpRequest "POST" "/internal/reviews/moderate"
+      | "Reviews.ModerationAccepted" => .httpResponse "Reviews.ModerateCommand"
+      | "Reviews.ModerationRejected" => .httpResponse "Reviews.ModerateCommand"
+      | "Reviews.PostResponse201" => .httpResponse "Reviews.PostRequest"
+      | "Reviews.PostResponse400" => .httpResponse "Reviews.PostRequest"
+      | _ => .custom "unassigned" ""
+  }
+
+def workerImplementation : LeanFM.ImplementationSpec :=
+  { requirementId := workerRequirement.id
+  , target := LeanFM.TargetLanguage.go
+  , moduleName := "example.com/leanfm/worker"
+  , outputDirectory := "generated/worker-go"
+  , actors := [WorkerActor.Client, WorkerActor.Gateway, WorkerActor.Worker].map actorBinding
+  , messages := workerRequirement.messages.map messageBinding
+  , channels :=
+      { sendFunction := "Send"
+      , receiveFunction := "Receive"
+      , tryReceiveFunction := "TryReceive"
+      , sendFull := LeanFM.SendFullSemantics.blockWithoutMutation
+      , receiveEmpty := LeanFM.ReceiveEmptySemantics.blockWithoutMutation
+      , tryReceiveEmpty := LeanFM.TryReceiveEmptySemantics.returnNoneKeepRunnable
+      }
+  }
+
+def validationReport : String :=
+  LeanFM.implementationValidationReport workerRequirement workerImplementation
+
+end LeanFM.LLMGenerated.Implementation
